certicoq/theories/L2_5_box/wcbvEval.v
@@ -1,3 +1,7 @@
+(****)
+Add LoadPath "../common" as Common.
+Add LoadPath "../L2_5_box" as L2_5.
+(****)
 
 Require Import Coq.Lists.List.
 Require Import Coq.Strings.String.
@@ -5,11 +9,11 @@ Require Import Coq.Arith.Compare_dec.
 Require Import Coq.Program.Basics.
 Require Import Coq.omega.Omega.
 Require Import Coq.Logic.JMeq.
-Require Import Common.AstCommon.
-Require Import L1g.term.
-Require Import L1g.program.
-Require Import L1g.wndEval.
-Require Import L1g.awndEval.
+Require Import Common.Common.
+Require Import L2_5.term.
+Require Import L2_5.program.
+Require Import L2_5.wndEval.
+Require Import L2_5.awndEval.
 
 Delimit Scope string_scope with string.
 Open Scope string_scope.
@@ -18,18 +22,14 @@ Open Scope bool.
 Open Scope list.
 Set Implicit Arguments.
 
+
 (** Big step relation of weak cbv evaluation  **)
 (** every field must evaluate **)
 Inductive WcbvEval (p:environ Term) : Term -> Term -> Prop :=
-| wPrf: forall t et, WcbvEval p t et -> WcbvEval p (TProof t) et
-| wLam: forall nm ty ty' bod,
-          WcbvEval p ty ty' ->
-          WcbvEval p (TLambda nm ty bod) (TLambda nm ty' bod)
-| wProd: forall nm ty ty' bod,
-          WcbvEval p ty ty' ->
-          WcbvEval p (TProd nm ty bod) (TProd nm ty' bod)
-| wCast: forall t s ty,
-           WcbvEval p t s ->  WcbvEval p (TCast t ty) s
+| wLam: forall nm bod, WcbvEval p (TLambda nm bod) (TLambda nm bod)
+| wProd: forall nm bod, WcbvEval p (TProd nm bod) (TProd nm bod)
+| wCast: forall t s, WcbvEval p t s ->  WcbvEval p (TCast t) s
+| wProof: WcbvEval p TProof TProof
 | wConstruct: forall i r arty,
                 WcbvEval p (TConstruct i r arty) (TConstruct i r arty)
 | wInd: forall i, WcbvEval p (TInd i) (TInd i) 
@@ -39,46 +39,39 @@ Inductive WcbvEval (p:environ Term) : Term -> Term -> Prop :=
 | wConst: forall nm (t s:Term),
             lookupDfn nm p = Ret t -> WcbvEval p t s ->
             WcbvEval p (TConst nm) s
-| wAppLam: forall (fn ty bod a1 a1' s:Term) (args:Terms) (nm:name),
-               WcbvEval p fn (TLambda nm ty bod) ->
+| wAppLam: forall (fn bod a1 a1' s:Term) (args:Terms) (nm:name),
+               WcbvEval p fn (TLambda nm bod) ->
                WcbvEval p a1 a1' ->
                WcbvEval p (whBetaStep bod a1' args) s ->
                WcbvEval p (TApp fn a1 args) s
-| wLetIn: forall (nm:name) (dfn ty bod dfn' s:Term),
+| wLetIn: forall (nm:name) (dfn bod dfn' s:Term),
             WcbvEval p dfn dfn' ->
             WcbvEval p (instantiate dfn' 0 bod) s ->
-            WcbvEval p (TLetIn nm dfn ty bod) s
-| wAppFix: forall dts m z (fn arg s x t t':Term)
-                  (args:Terms) (ix:nat),
+            WcbvEval p (TLetIn nm dfn bod) s
+| wAppFix: forall dts m (fn arg s x:Term) (args:Terms) (ix:nat),
              WcbvEval p fn (TFix dts m) ->
              dnthBody m dts = Some (x, ix) ->
-             (***
-             tsplit ix (tcons arg args) = Some  (mkSplit brfsts t brlsts) ->
-              ***)
-             tnth ix (tcons arg args) = Some t ->
-             WcbvEval p t t' ->
-             canonicalP t' = Some z ->   (* test Fix is guarded *)
              WcbvEval p (pre_whFixStep x dts (tcons arg args)) s ->
              WcbvEval p (TApp fn arg args) s
-| wAppCong: forall fn fn' arg args arg' args',
+| wAppCong: forall fn fn' arg args arg' args' s,
               WcbvEval p fn fn' ->
               ~ isLambda fn' -> ~ isFix fn' ->
               WcbvEvals p (tcons arg args) (tcons arg' args') ->
-              WcbvEval p (TApp fn arg args) (mkApp fn' (tcons arg' args'))
-| wCase: forall mch Mch n args ml ts brs cs s ty arty,
+              (mkApp fn' (tcons arg' args')) = s ->
+              WcbvEval p (TApp fn arg args) s
+| wCase: forall mch Mch n args ml ts brs cs s arty,
                 WcbvEval p mch Mch ->
                 canonicalP Mch = Some (n, args, arty) ->
                 tskipn (snd (fst ml)) args = Some ts ->
                 whCaseStep n ts brs = Some cs ->
                 WcbvEval p cs s ->
-                WcbvEval p (TCase ml ty mch brs) s
-| wCaseCong: forall mch Mch ty ty' ml brs brs',
+                WcbvEval p (TCase ml mch brs) s
+| wCaseCong: forall mch Mch ml brs brs',
              WcbvEval p mch Mch ->
              canonicalP Mch = None ->
-             WcbvEval p ty ty' ->
              WcbvEvals p brs brs' ->           
-             WcbvEval p (TCase ml ty mch brs) (TCase ml ty' Mch brs')
-| wWrong: forall str, WcbvEval p (TWrong str) (TWrong str)
+             WcbvEval p (TCase ml mch brs) (TCase ml Mch brs')
+| wWrong: WcbvEval p TWrong TWrong
 with WcbvEvals (p:environ Term) : Terms -> Terms -> Prop :=
 | wNil: WcbvEvals p tnil tnil
 | wCons: forall t t' ts ts',
@@ -89,21 +82,50 @@ Scheme WcbvEval1_ind := Induction for WcbvEval Sort Prop
      with WcbvEvals1_ind := Induction for WcbvEvals Sort Prop.
 Combined Scheme WcbvEvalEvals_ind from WcbvEval1_ind, WcbvEvals1_ind.
 
-
 (** evaluate omega = (\x.xx)(\x.xx): nontermination **)
-Definition xx := (TLambda nAnon prop (TApp (TRel 0) (TRel 0) tnil)).
+Definition xx := (TLambda nAnon (TApp (TRel 0) (TRel 0) tnil)).
 Definition xxxx := (TApp xx xx tnil).
 Goal WcbvEval nil xxxx xxxx.
 unfold xxxx, xx.
-eapply wAppLam. eapply wLam. eapply wSort. 
-eapply wLam. eapply wSort. 
-unfold whBetaStep, instantiate.
-rewrite (proj2 (nat_compare_eq_iff 0 0) eq_refl).
-rewrite mkApp_idempotent. simpl. 
+eapply wAppLam. eapply wLam. 
+eapply wLam. 
 change (WcbvEval nil xxxx xxxx).
 Abort.
 
 
+Lemma isL2_5Cnstr_WcbvEval_TCnstr:
+  forall t i x arty, isL2_5Cnstr t = Some (i, x, arty) ->
+                     forall p u, WcbvEval p t u -> u = TConstruct i x arty.
+Proof.
+  intros t.
+  functional induction (isL2_5Cnstr t); intros; try discriminate.
+  - myInjection H. inversion_Clear H0. reflexivity.
+  - eapply IHo. assumption. inversion_Clear H0. eassumption.
+Qed.
+
+Lemma isL2_5Cnstr_WcbvEval_TApp:
+  forall t i x arty, isL2_5Cnstr t = Some (i, x, arty) ->
+                     forall p et, WcbvEval p t et ->
+  forall arg args earg eargs,
+    WcbvEval p arg earg -> WcbvEvals p args eargs ->
+    WcbvEval p (TApp t arg args) (TApp (TConstruct i x arty) earg eargs).
+Proof.
+  intros t.
+  functional induction (isL2_5Cnstr t); intros; try discriminate.
+  - myInjection H. eapply wAppCong. constructor. 
+    + not_isLambda.
+    + not_isFix.
+    + intuition. eapply wCons; eassumption.
+    + rewrite <- (mkApp_goodFn _  eargs). reflexivity. not_isApp.
+  - inversion_Clear H0. assert (j:= isL2_5Cnstr_WcbvEval_TCnstr H H4).
+    rewrite j in H4.
+    eapply wAppCong; try eassumption. eapply wCast. eassumption.
+    + not_isLambda.
+    + not_isFix.
+    + eapply wCons; eassumption.
+    + rewrite <- (mkApp_goodFn _  eargs). reflexivity. not_isApp.
+Qed.
+            
 Lemma WcbvEval_mkApp_nil:
   forall t, WFapp t -> forall p s, WcbvEval p t s ->
                  WcbvEval p (mkApp t tnil) s.
@@ -111,7 +133,6 @@ Proof.
   intros p. induction 1; simpl; intros; try assumption.
   - rewrite tappend_tnil. assumption.
 Qed.
-
 
 (*******  move to somewhere  ********)
 Lemma lookup_pres_WFapp:
@@ -123,7 +144,7 @@ Proof.
     + cbn in h. rewrite j in h. myInjection h. assumption.
     + cbn in h. rewrite j in h. eapply IHWFaEnv. eassumption.
 Qed.
-
+  
 (**************************************************)
 
 (** wcbvEval preserves WFapp **)
@@ -135,8 +156,7 @@ Proof.
   intros p hp.
   apply WcbvEvalEvals_ind; intros; try assumption;
   try (solve[inversion_Clear H0; intuition]);
-  try (solve[inversion_Clear H1; intuition]);
-  try (solve[inversion_Clear H2; intuition]).
+  try (solve[inversion_Clear H1; intuition]).
   - apply H. unfold lookupDfn in e. case_eq (lookup nm p); intros xc.
     + intros k. assert (j:= lookup_pres_WFapp hp _ k)
       . rewrite k in e. destruct xc. 
@@ -148,12 +168,12 @@ Proof.
     apply (whBetaStep_pres_WFapp); intuition. 
   - inversion_Clear H1. apply H0. apply instantiate_pres_WFapp. assumption.
     + apply H. assumption.
-  - inversion_clear H2. apply H1.
-    specialize (H H4). inversion_Clear H.
+  - inversion_clear H1. apply H0.
+    specialize (H H3). inversion_Clear H.
     apply pre_whFixStep_pres_WFapp; try assumption.
-    + apply (dnthBody_pres_WFapp H7 _ e).
+    + apply (dnthBody_pres_WFapp H6 _ e).
     + constructor; assumption.
-  - inversion_Clear H1.
+   - inversion_Clear H1.
     destruct (mkApp_isApp_lem fn' arg' args') as
         [y0 [y1 [y2 [ka [[kc1 [kc2 [kc3 kc4]]] | [kd1 [kd2 kd3]]]]]]];
       rewrite ka.
@@ -168,7 +188,7 @@ Proof.
       rewrite <- tappend_assoc. cbn. apply tappend_pres_WFapps; try assumption.
       apply H0. constructor; try assumption.
   - apply H0. inversion_Clear H1. 
-    refine (whCaseStep_pres_WFapp H7 _ _ e1). 
+    refine (whCaseStep_pres_WFapp H6 _ _ e1). 
     refine (tskipn_pres_WFapp _ _ e0).
     refine (canonicalP_pres_WFapp _ e). intuition.
 Qed.
@@ -181,24 +201,23 @@ Lemma WcbvEval_weaken:
                    WcbvEvals ((nm,ec)::p) ts ss).
 Proof.
   intros p. apply WcbvEvalEvals_ind; intros; auto.
-   - destruct (string_dec nm nm0).
-    + subst. inversion_Clear H0.
+  - destruct (string_dec nm nm0).
+    + subst. 
       * unfold lookupDfn in e.
-        rewrite (proj1 (fresh_lookup_None (trm:=Term) _ _)) in e.
+        rewrite (proj1 (fresh_lookup_None (trm:=Term) _ _) H0) in e.
         discriminate.
-        constructor; assumption.
-      * unfold lookupDfn in e.
-        rewrite (proj1 (fresh_lookup_None (trm:=Term) _ _)) in e.
-        discriminate.  constructor.
     + eapply wConst.
       * rewrite <- (lookupDfn_weaken' n). eassumption. 
       * apply H. assumption. 
-   - eapply wAppLam.
+  - eapply wAppLam.
     + apply H. assumption.
     + apply H0. assumption.
     + apply H1. assumption.
   - eapply wLetIn; intuition.
   - eapply wAppFix; try eassumption; intuition.
+  - eapply wAppCong; try eassumption.
+    + eapply H. assumption.
+    + eapply H0. assumption.
   - eapply wCase; intuition; eassumption.
 Qed.
 
@@ -216,38 +235,38 @@ Lemma WcbvEvals_tcons_tcons':
 Proof.
   inversion 1. intuition.
 Qed.
+ 
+(****  Could probably finish this, bus see WcbvEval_wndEvalRTC below ***
+(** WcbvEval is in the transitive closure of wndEval **)
+Lemma WcbvEval_wndEvalTC:
+  forall (p:environ), WFaEnv p ->
+    (forall t s, WcbvEval p t s -> t <> s ->
+        WFapp t -> wndEvalTC p t s) /\
+    (forall ts ss, WcbvEvals p ts ss -> ts <> ss ->
+        WFapps ts -> wndEvalsTC p ts ss).
+Proof.
+  intros p hp. apply WcbvEvalEvals_ind; intros; try (nreflexivity H).
+Qed.
+*******)
 
-(****************
 Lemma WcbvEval_wndEvalRTC:
   forall (p:environ Term), WFaEnv p ->
-    (forall t s, WcbvEval p t s -> WFapp t -> wndEvalRTC p t s) /\
-    (forall ts ss, WcbvEvals p ts ss -> WFapps ts -> wndEvalsRTC p ts ss).
+   (forall t s, WcbvEval p t s -> WFapp t -> wndEvalRTC p t s) /\
+   (forall ts ss, WcbvEvals p ts ss -> WFapps ts -> wndEvalsRTC p ts ss).
 Proof.
   intros p hp. apply WcbvEvalEvals_ind; intros; try (solve [constructor]).
-  - eapply wERTCtrn; inversion_Clear H0.
-    + apply wERTCstep. apply sPrf.
-    + apply H. assumption.
-  - inversion_Clear H0. 
-    eapply wERTCtrn. 
-    + apply wndEvalRTC_Lam_typ. eapply H. assumption.
-    + constructor. 
-  - inversion_Clear H0. 
-    eapply wERTCtrn. 
-    + apply wndEvalRTC_Prod_typ. eapply H. assumption.
-    + constructor. 
-  - eapply wERTCtrn; inversion_Clear H0.
-    + apply wERTCstep. apply sCast.
-    + apply H. assumption.
-   - eapply wERTCtrn; intuition.
+  - eapply wERTCtrn. apply wERTCstep. apply sCast. apply H. 
+    inversion_Clear H0. assumption.
+  - eapply wERTCtrn; intuition.
     eapply wERTCtrn.
     + apply wERTCstep. apply sConst. apply lookupDfn_LookupDfn. eassumption.
-    + apply H. eapply (lookupDfn_pres_WFapp hp).  eassumption. 
+    + apply H. eapply (lookupDfn_pres_WFapp hp).  eassumption.
   - inversion_Clear H2.
-    eapply (@wERTCtrn _ _ (TApp (TLambda nm ty bod) a1 args)).
+    eapply (@wERTCtrn _ _ (TApp (TLambda nm bod) a1 args)).
     + rewrite <- mkApp_goodFn; try assumption.
       rewrite <- mkApp_goodFn; try not_isApp.
       apply wndEvalRTC_App_fn; try assumption. intuition.
-    + eapply (@wERTCtrn _ _ (TApp (TLambda nm ty bod) a1' args)).
+    + eapply (@wERTCtrn _ _ (TApp (TLambda nm bod) a1' args)).
       * eapply wndEvalRTC_App_arg; try reflexivity.
         apply H0. assumption.
       * { apply (@wERTCtrn _ _ (whBetaStep bod a1' args)).
@@ -256,14 +275,14 @@ Proof.
             + assert (j:= proj1 (wcbvEval_pres_WFapp hp) _ _ w H7).
               inversion_Clear j. assumption.
             + apply (proj1 (wcbvEval_pres_WFapp hp) _ _ w0 H8). }
-  - inversion_Clear H1. eapply (@wERTCtrn _ _ (TLetIn nm dfn' ty bod)).
+  - inversion_Clear H1. eapply (@wERTCtrn _ _ (TLetIn nm dfn' bod)).
     + apply wndEvalRTC_LetIn_dfn. intuition.
     + eapply wERTCtrn. apply wERTCstep. apply sLetIn. apply H0.
       apply instantiate_pres_WFapp; try assumption.
       * eapply (proj1 (wcbvEval_pres_WFapp hp)); try eassumption.
-  - inversion_clear H2. specialize (H H4).
+  - inversion_clear H1. specialize (H H3).
     assert (j0: WFapps (tcons arg args)).
-    { constructor; assumption. }
+    { constructor; eassumption. }
     assert (j2: WFapp (TFix dts m)).
     { refine (proj1 (wcbvEval_pres_WFapp hp) _ _ w _). assumption. }
     inversion_clear j2.
@@ -271,22 +290,13 @@ Proof.
     { refine (dnthBody_pres_WFapp _ _ e). assumption. }
     assert (j4: WFapp (pre_whFixStep x dts (tcons arg args))).
     { refine (pre_whFixStep_pres_WFapp _ _ _); assumption. }
-    specialize (H1 j4).
+    specialize (H0 j4).
     refine (@wERTCtrn _ _ (TApp (TFix dts m) arg args) _ _ _).
     + rewrite <- mkApp_goodFn; try assumption.
       rewrite <- mkApp_goodFn; try not_isApp.
       apply wndEvalRTC_App_fn; assumption.
-    + (* destruct (WcbvEvals_tcons_tcons w0) as [x0 [x1 j]]. subst. *)
-      eapply (@wERTCtrn _ _ (pre_whFixStep x dts (tcons arg args)));
-      try assumption.
-      * eapply wERTCstep. eapply sFix; try eassumption.
-
-        
-      refine (wndEvalsRTC_App_args _ eq_refl eq_refl _); try not_isApp.
-      intuition.
-      refine (wERTCtrn _ H1).
-      eapply wERTCtrn.
-      * eapply wndEvalsRTC_Fix. eapply sFix; try eassumption.
+    + eapply wERTCtrn; try eassumption.
+      apply wERTCstep. eapply sFix; eassumption.
   - inversion_Clear H1. specialize (H H6). specialize (H0 (wfacons H7 H8)).
     eapply (@wERTCtrn _ _ (TApp fn arg' args')).
     + eapply wndEvalsRTC_App_args; try reflexivity; try assumption.
@@ -303,74 +313,33 @@ Proof.
       * { apply H0. refine (whCaseStep_pres_WFapp _ _ _ e1). assumption.
           refine (tskipn_pres_WFapp _ _ e0).
           refine (canonicalP_pres_WFapp _ e).
-          specialize (H H5).
+          specialize (H H4).
           refine (wndEvalRTC_pres_WFapp _ _ _); eassumption. }
-  - inversion_Clear H2. eapply wERTCtrn.
+  - inversion_Clear H1. eapply wERTCtrn.
     + eapply wndEvalRTC_Case_mch. apply H. assumption.
-    + eapply (@wERTCtrn _ _  (TCase ml ty' Mch brs)).
-      * apply wndEvalRTC_Case_ty. intuition.
-      * eapply (@wERTCtrn _ _  (TCase ml ty' Mch brs')).
+    + eapply (@wERTCtrn _ _  (TCase ml Mch brs)).
+      * apply wERTCrfl. 
+      * eapply (@wERTCtrn _ _  (TCase ml Mch brs')).
         apply wndEvalRTC_Case_brs. intuition.
         constructor.
   - inversion_Clear H1. eapply (@wEsRTCtrn _ _ (tcons t' ts)).
     + apply wndEvalsRTC_tcons_hd. apply H. assumption.
     + apply wndEvalsRTC_tcons_tl. apply H0. assumption.
 Qed.
-**********************)
 
-
-(*************************
-Goal
-  forall t, WFapp t ->
-            forall fn arg args, t = (mkApp fn (tcons arg args)) ->
-                                WFapp fn /\ WFapp arg /\ WFapps args.
-Proof.
-  induction 1; intros; destruct (mkApp_isApp fn arg args) as [y [y0 [y1 jy]]];
-  try (solve[rewrite jy in *;  discriminate]).
-  - rewrite mkApp_goodFn in jy; try assumption. myInjection jy.
-    apply IHWFapp1.
-  
+(*****
 Lemma wcbvEval_no_further:
   forall p,
-    (forall t s, WcbvEval p t s -> WFapp s -> WcbvEval p s s) /\
-    (forall ts ss, WcbvEvals p ts ss -> WFapps ss -> WcbvEvals p ss ss).
+  (forall t s, WcbvEval p t s -> WcbvEval p s s) /\
+  (forall ts ss, WcbvEvals p ts ss -> WcbvEvals p ss ss).
 Proof.
   intros p.
-  apply WcbvEvalEvals_ind; cbn; intros. Focus 13.
-  - Check mkApp_pres_WFapp.
-  
-  try inversion_Clear H0; try inversion_Clear H1;
-  try (solve [constructor; intuition]); intuition;
-  try (assert (j:= mkApp_isApp fn' arg' args');
-       destruct j as [x0 [x1 [x2 k]]]; rewrite k in *; discriminate).
-  - rewrite mkApp_goodFn in H2.
-    + myInjection H2.
-      rewrite <- mkApp_goodFn at 2; try assumption.
-      apply wAppCong; intuition.
-    + intros h. destruct h as [y0 [y1 [y2 ky]]]. rewrite ky in H2.
-      cbn in H2. myInjection H2.
-
-  - rewrite <- mkApp_goodFn at 2; try assumption.
-    apply wAppCong; try assumption.
-    
-  - destruct (mkApp_isApp_lem fn' arg' args') as
-        [y0 [y1 [y2 [ka [[kc1 [kc2 [kc3 kc4]]] | [kd1 [kd2 kd3]]]]]]].
-    + subst. rewrite <- mkApp_goodFn at 2; try assumption.
-      apply wAppCong; try assumption.
-      rewrite ka.
-
-
-Check (mkApp_isApp_lem fn' arg' args').
-    
-  - admit. (** rewrite H2 at 2. apply wAppCong; try assumption. *)
-  - inversion_Clear H2.
-    specialize (H1 H8). specialize (H0 H9). specialize (H H6).
-    eapply wCaseCong; try eassumption.
+  apply WcbvEvalEvals_ind; simpl; intros; auto.
 Qed.
- *********************)
+*****)
 
 Section wcbvEval_sec.
-Variable p : environ Term.
+Variable p:environ Term.
 
 Function wcbvEval
          (tmr:nat) (t:Term) {struct tmr}: exception Term :=
@@ -378,19 +347,15 @@ Function wcbvEval
     | 0 => raise ("out of time: " ++ print_term t)
     | S n =>
       match t with      (** look for a redex **)
-        | TProof t =>
-          match wcbvEval n t with
-            | Ret et => Ret et
-            | _ => raise ("wcbvEval: TProof")
-          end
         | TConst nm =>
           match (lookup nm p) with
             | Some (AstCommon.ecTrm t) => wcbvEval n t
                   (** note hack coding of axioms in environment **)
-            | Some _ => raise ("wcbvEval, TConst ecTyp " ++ nm)
-            | _ => raise ("wcbvEval: TConst environment miss:  " ++ nm)
+            | Some (AstCommon.ecTyp _ _ _) =>
+              raise ("wcbvEval, TConst ecTyp " ++ nm)
+            | _ => raise "wcbvEval: TConst environment miss"
           end
-        | TCast t _ =>
+        | TCast t =>
           match wcbvEval n t with
             | Ret et => Ret et
             | Exc s => raise ("wcbvEval: TCast: " ++ s)
@@ -398,48 +363,33 @@ Function wcbvEval
         | TApp fn a1 args =>
           match wcbvEval n fn with
             | Exc s => raise ("wcbvEval TApp: fn doesn't eval: " ++ s)
-            | Ret (TLambda _ _ bod) =>
+            | Ret (TLambda _ bod) =>
               match wcbvEval n a1 with
                 | Exc s =>  raise ("wcbvEval TApp: arg doesn't eval: " ++ s)
                 | Ret b1 => wcbvEval n (whBetaStep bod b1 args)
               end
+            | Ret (TFix dts m) =>
+              match dnthBody m dts with
+                | None =>
+                  raise ("wcbvEval TApp: dnthBody doesn't eval")
+                | Some (x, ix) =>
+                  wcbvEval n (pre_whFixStep x dts (tcons a1 args))
+              end
             | Ret Fn =>
               match wcbvEvals n (tcons a1 args) with
                 | Exc s => raise ("wcbvEval TApp: args don't eval: " ++ s)
-                | Ret ergs =>
-                  match Fn with
-                    | TFix dts m =>  
-                      match dnthBody m dts with
-                        | None =>
-                          raise ("wcbvEval TApp: dnthBody doesn't eval: ")
-                        | Some (x, ix) =>
-                          match tnth ix ergs with
-                            | None => raise ("wcbvEval TApp: tnth not defined")
-                            | Some t =>
-                              match canonicalP t with (* test Fix is guarded *)
-                                | Some _ =>
-                                  wcbvEval n (pre_whFixStep x dts ergs)
-                                | None => raise ("wcbvEval TFix: rec arg ")
-                              end
-                          end
-                      end
-                    | Fn => ret (mkApp Fn ergs)
-                  end
+                | Ret ergs => ret (mkApp Fn ergs)
               end
           end
-        | TCase ml tp mch brs =>
+        | TCase ml mch brs =>
           match wcbvEval n mch with
             | Exc str => Exc str
             | Ret emch =>
               match canonicalP emch with
                 | None =>
-                  match wcbvEval n tp with
-                    | Exc str => Exc str
-                    | Ret etp =>
-                      match wcbvEvals n brs with
-                        | Exc _ => Exc ("wcbvEval; TCase, brs don't eval")
-                        | Ret ebrs => Ret (TCase ml etp emch ebrs)
-                      end
+                  match wcbvEvals n brs with
+                    | Exc _ => Exc ("wcbvEval; TCase, brs don't eval")
+                    | Ret ebrs => Ret (TCase ml emch ebrs)
                   end
                 | Some (r, args, _) =>
                   match tskipn (snd (fst ml)) args with
@@ -452,53 +402,44 @@ Function wcbvEval
                   end
               end
           end
-        | TLetIn nm df _ bod =>
+        | TLetIn nm df bod =>
           match wcbvEval n df with
             | Ret df' => wcbvEval n (instantiate df' 0 bod)
             | Exc s => raise ("wcbvEval: TLetIn: " ++ s)
           end
-        | TLambda nn ty t => 
-          match wcbvEval n ty with
-            | Exc str => Exc str
-            | Ret ty' => ret (TLambda nn ty' t)
-          end
-        | TProd nn ty t =>
-          match wcbvEval n ty with
-            | Exc str => Exc str
-            | Ret ty' => ret (TProd nn ty' t)
-          end
         (** already in whnf ***)
         | TAx => ret TAx
+        | TLambda nn t => ret (TLambda nn t)
+        | TProd nn t => ret (TProd nn t)
         | TFix mfp br => ret (TFix mfp br)
         | TConstruct i cn arty => ret (TConstruct i cn arty)
         | TInd i => ret (TInd i)
         | TSort srt => ret (TSort srt)
+        | TProof => ret TProof
         (** should never appear **)
         | TRel _ => raise "wcbvEval: unbound Rel"
-        | TWrong str => ret (TWrong str)
+        | TWrong => ret TWrong
       end
   end
-with wcbvEvals (tmr:nat) (ts:Terms) {struct tmr} : exception Terms :=
-       match tmr with 
-         | 0 => raise "out of time"
-         | S n => match ts with             (** look for a redex **)
-                    | tnil => ret tnil
-                    | tcons s ss =>
-                      match wcbvEval n s with
-                        | Exc s => raise ("wcbEvals: tconsl " ++ s)
-                        | Ret es =>
-                          match wcbvEvals n ss with
-                            | Exc s => raise ("wcbEvals: tconsr " ++ s)
-                            | Ret ess => ret (tcons es ess)
-                          end
-                      end
-                  end
-       end.
+with wcbvEvals (tmr:nat) (ts:Terms) {struct tmr}
+     : exception Terms :=
+       (match tmr with 
+          | 0 => raise "out of time"
+          | S n => match ts with             (** look for a redex **)
+                     | tnil => ret tnil
+                     | tcons s ss =>
+                       match wcbvEval n s, wcbvEvals n ss with
+                         | Ret es, Ret ess => ret (tcons es ess)
+                         | Exc s, _ => raise s
+                         | Ret _, Exc s => raise s
+                       end
+                   end
+        end).
 Functional Scheme wcbvEval_ind' := Induction for wcbvEval Sort Prop
 with wcbvEvals_ind' := Induction for wcbvEvals Sort Prop.
 Combined Scheme wcbvEvalEvals_ind from wcbvEval_ind', wcbvEvals_ind'.
 
-(**************  fix ******************
+
 (** wcbvEval and WcbvEval are the same relation **)
 Lemma wcbvEval_WcbvEval:
   forall tmr,
@@ -515,23 +456,20 @@ Proof.
     + unfold lookupDfn. rewrite e1. reflexivity.
   - specialize (H1 _ p1). specialize (H _ e1). specialize (H0 _ e2).
     eapply wAppLam; eassumption.
-  - specialize (H1 _ p1). specialize (H _ e1). specialize (H0 _ e2).
-    destruct (isFix_dec Fn); subst.
-    + destruct (WcbvEvals_tcons_tcons H0) as [g0 [g1 hg]]. subst.
-      refine (wAppFix _ _ _ _ _ _); try eassumption.
-    + elim n0. auto.
-  - specialize (H _ e1). specialize (H0 _ e2).
+  - specialize (H0 _ p1). specialize (H _ e1). subst.
+    eapply wAppFix; try eassumption.
+  - specialize (H _ e1). specialize (H0 _ e2). 
     destruct (WcbvEvals_tcons_tcons H0) as [g0 [g1 hg]]. subst.
     eapply wAppCong; try eassumption.
-    + destruct Fn0; try not_isLambda. auto.
-    + destruct Fn0; try not_isFix. auto.
+    + destruct Fn; try not_isLambda. contradiction.
+    + destruct Fn; try not_isFix. contradiction.
+    + reflexivity.
   - eapply wCase; try eassumption.
     + apply H; eassumption.
     + apply H0; eassumption. 
   - eapply wLetIn; intuition.
     + apply H. assumption.
 Qed.
-
 
 (** need strengthening to large-enough fuel to make the induction
  *** go through **)
@@ -541,21 +479,17 @@ Lemma pre_WcbvEval_wcbvEval:
     (forall ts ss, WcbvEvals p ts ss ->
                    exists n, forall m, m >= n -> wcbvEvals (S m) ts = Ret ss).
 Proof.
-  assert (j:forall m x, m > x -> m = S (m - 1)). { induction m; intuition. }
-                                                 apply WcbvEvalEvals_ind; intros; try (exists 0; intros mx h; reflexivity).
-  - destruct H. exists (S x). intros m hm. simpl. rewrite (j m x); try omega.
-    + rewrite (H (m - 1)); try omega. reflexivity. 
+  assert (j:forall m x, m > x -> m = S (m - 1)).
+  { induction m; intuition. }
+  apply WcbvEvalEvals_ind; intros; try (exists 0; intros mx h; reflexivity).
   - destruct H. exists (S x). intros m hm. simpl. rewrite (j m x); try omega.
     + rewrite (H (m - 1)); try omega. reflexivity.
-  - destruct H.  exists (S x). intros m h. simpl.
-    rewrite (j m x); try omega. rewrite H; try omega. reflexivity.
-  - destruct H. exists (S x). intros mm h. cbn. 
-    rewrite (j mm x); try omega. rewrite H. reflexivity. omega.
-  - destruct H. exists (S x). intros mm h. cbn.
+  - destruct H. exists (S x). intros mm h. simpl.
     rewrite (j mm x); try omega.
-    unfold lookupDfn in e. destruct (lookup nm p); try discriminate.
-    + destruct e0; try discriminate. myInjection e. rewrite H.
-      reflexivity. omega.
+    unfold lookupDfn in e. destruct (lookup nm p). destruct e0. myInjection e.
+    + rewrite H. reflexivity. omega.
+    + discriminate.
+    + discriminate.
   - destruct H, H0, H1. exists (S (max x (max x0 x1))). intros m h.
     assert (j1:= max_fst x (max x0 x1)). 
     assert (lx: m > x). omega.
@@ -565,7 +499,7 @@ Proof.
     assert (j4:= max_snd x0 x1).
     assert (j5:= max_fst x0 x1).
     assert (lx1: m > x1). omega.
-    assert (k:wcbvEval m fn = Ret (TLambda nm ty bod)).
+    assert (k:wcbvEval m fn = Ret (TLambda nm bod)).
     + rewrite (j m (max x (max x0 x1))). apply H.
       assert (l:= max_fst x (max x0 x1)); omega. omega.
     + assert (k0:wcbvEval m a1 = Ret a1').
@@ -579,24 +513,15 @@ Proof.
     assert (l1:= max_fst x x0). assert (l2:= max_snd x x0).
     simpl. rewrite (j mx x); try omega. rewrite (H (mx - 1)); try omega.
     rewrite H0; try omega. reflexivity.
-  - destruct H, H0, H1. exists (S (max x0 (max x1 x2))). intros mx h.
-    assert (j1:= max_fst x0 (max x1 x2)). 
-    assert (lx: mx > x0). omega.
-    assert (j2:= max_snd x0 (max x1 x2)).
-    assert (j3:= max_fst x1 x2).
-    assert (lx0: mx > x1). omega.
-    assert (j4:= max_snd x1 x2).
-    assert (j5:= max_fst x1 x2).
-    assert (lx1: mx > x2). omega.
-    destruct (WcbvEvals_tcons_tcons w0) as [y0 [y1 k0]].
-    simpl. rewrite (j mx x0); try omega. rewrite H0; try omega.
-    rewrite k0 in *. rewrite H; try omega. rewrite e. rewrite e0. rewrite e1.
-    apply H1. omega.
+  - destruct H, H0. exists (S (max x0 x1)). intros mx h.
+    assert (l1:= max_fst x0 x1). assert (l2:= max_snd x0 x1).
+    cbn. rewrite (j mx x0); try omega. rewrite (H (mx - 1)); try omega.
+    rewrite e. rewrite H0. reflexivity. omega. 
   - destruct H, H0. exists (S (max x x0)). intros mx h.
     assert (l1:= max_fst x x0). assert (l2:= max_snd x x0).
     cbn. rewrite (j mx x); try omega. rewrite (H0 (mx - 1)); try omega.
     rewrite (H (mx - 1)); try omega.
-    destruct fn'; try reflexivity.
+    destruct fn'; try reflexivity; repeat (try (apply f_equal; assumption)).
     + elim n; auto.
     + elim n0; auto.
   - destruct H, H0. exists (S (max x x0)). intros mx h.
@@ -604,20 +529,11 @@ Proof.
     cbn. rewrite (j mx x); try omega. rewrite (H (mx - 1)); try omega.
     rewrite e. rewrite e0. rewrite e1. rewrite (H0 (mx - 1)); try omega.
     reflexivity.
-  - destruct H as [x0 jx0], H0 as [x1 jx1], H1 as [x2 jx2].
-    exists (S (max x0 (max x1 x2))). intros mx h.
-    assert (j1:= max_fst x0 (max x1 x2)). 
-    assert (lx: mx > x0). omega.
-    assert (j2:= max_snd x0 (max x1 x2)).
-    assert (j3:= max_fst x1 x2).
-    assert (lx0: mx > x1). omega.
-    assert (j4:= max_snd x1 x2).
-    assert (j5:= max_fst x1 x2).
-    assert (lx1: mx > x2). omega.
-    simpl. rewrite (j mx x0); try omega.
-    rewrite jx0; try omega. rewrite e.
-    rewrite jx1; try omega.
-    rewrite jx2; try omega. reflexivity.
+  - destruct H, H0. exists (S (max x x0)). intros mx h.
+    assert (l1:= max_fst x x0). assert (l2:= max_snd x x0).
+    cbn. rewrite (j mx x); try omega. rewrite (H (mx - 1)); try omega.
+    rewrite e. rewrite H0; try omega.
+    reflexivity.
   - destruct H, H0. exists (S (max x x0)). intros mx h.
     assert (l1:= max_fst x x0). assert (l2:= max_snd x x0).
     simpl. rewrite (j mx x); try omega. rewrite (H (mx - 1)); try omega.
