certicoq/theories/L2_5_box/compile.v
@@ -1,0 +1,216 @@
+
+(****)
+Add LoadPath "../common" as Common.
+Add LoadPath "../L2_typeStripped" as L2.
+(****)
+
+Require Import Coq.Lists.List.
+Require Import Coq.Strings.String.
+Require Import Coq.Arith.Compare_dec.
+Require Export Template.Ast.
+Require Import Common.Common.
+Require Import L2.compile.
+
+
+Local Open Scope string_scope.
+Local Open Scope bool.
+Local Open Scope list.
+Set Implicit Arguments.
+
+Definition L2Term := L2.compile.Term.
+Definition L2Terms := L2.compile.Terms.
+Definition L2Defs := L2.compile.Defs.
+Definition L2EC := envClass L2Term.
+Definition L2Env := environ L2Term.
+Definition L2Pgm := Program L2Term.
+
+
+Inductive Term : Type :=
+| TRel       : nat -> Term
+| TSort      : Srt -> Term
+| TProof     : Term
+| TCast      : Term -> Term
+| TProd      : name -> Term -> Term
+| TLambda    : name -> Term -> Term
+| TLetIn     : name ->
+               Term (* dfn *) -> Term (* body *) -> Term
+| TApp       : Term -> Term (* first arg must exist *) -> Terms -> Term
+| TConst     : string -> Term
+| TAx        : Term
+| TInd       : inductive -> Term
+| TConstruct : inductive -> nat (* index in datatype *) ->
+               nat (* arity *) -> Term
+| TCase      : (inductive * nat * list nat) (* # params, args per branch *) ->
+               Term -> Terms -> Term
+| TFix       : Defs -> nat -> Term
+| TWrong     : Term
+with Terms : Type :=
+| tnil : Terms
+| tcons : Term -> Terms -> Terms
+with Defs : Type :=
+| dnil : Defs
+| dcons : name -> Term -> nat -> Defs -> Defs.
+Hint Constructors Term Terms Defs.
+Scheme Trm_ind' := Induction for Term Sort Prop
+  with Trms_ind' := Induction for Terms Sort Prop
+  with Defs_ind' := Induction for Defs Sort Prop.
+Combined Scheme TrmTrmsDefs_ind from Trm_ind', Trms_ind', Defs_ind'.
+Combined Scheme TrmTrms_ind from Trm_ind', Trms_ind'.
+Notation prop := (TSort SProp).
+Notation set_ := (TSort SSet).
+Notation type_ := (TSort SType).
+Notation tunit t := (tcons t tnil).
+
+
+(*** \box in case branches: need tappend, mkApp and instantiate ***)
+Function tappend (ts1 ts2:Terms) : Terms :=
+  match ts1 with
+    | tnil => ts2
+    | tcons t ts => tcons t (tappend ts ts2)
+  end.
+Fixpoint dlength (ts:Defs) : nat :=
+  match ts with 
+    | dnil => 0
+    | dcons _ _ _ ts => S (dlength ts)
+  end.
+(** syntactic control of "TApp": no nested apps, app must have an argument **)
+Function mkApp (t:Term) (args:Terms) {struct t} : Term :=
+  match t with
+    | TApp fn b bs => TApp fn b (tappend bs args)
+    | fn => match args with
+              | tnil => fn
+              | tcons c cs => TApp fn c cs
+            end
+  end.
+Section Instantiate_sec.
+Variable (tin:Term).
+Function instantiate (n:nat) (tbod:Term) {struct tbod} : Term :=
+  match tbod with
+    | TRel m => match nat_compare n m with
+                  | Datatypes.Eq => tin
+                  | Gt => TRel m
+                  | Lt => TRel (pred m)
+                end
+    | TApp t a ts =>
+      mkApp (instantiate n t) (tcons (instantiate n a) (instantiates n ts))
+    | TLambda nm  bod =>
+      TLambda nm  (instantiate (S n) bod)
+    | TProd nm bod => TProd nm (instantiate (S n) bod)
+    | TCase np s ts =>
+      TCase np (instantiate n s) (instantiates n ts)
+    | TLetIn nm tdef bod =>
+      TLetIn nm (instantiate n tdef) (instantiate (S n) bod)
+    | TFix ds m => TFix (instantiateDefs (n + dlength ds) ds) m
+    | TCast t => instantiate n t
+    | x => x
+  end
+with instantiates (n:nat) (args:Terms) {struct args} : Terms :=
+       match args with
+         | tnil => tnil
+         | tcons t ts => tcons (instantiate n t) (instantiates n ts)
+       end
+with instantiateDefs (n:nat) (ds:Defs) {struct ds} : Defs :=
+       match ds with
+         | dnil => dnil
+         | dcons nm bod rarg ds =>
+           dcons nm (instantiate n bod) rarg (instantiateDefs n ds)
+       end.
+Functional Scheme instantiate_ind' := Induction for instantiate Sort Prop
+with instantiates_ind' := Induction for instantiates Sort Prop
+with instantiateDefs_ind' := Induction for instantiateDefs Sort Prop.
+End Instantiate_sec.
+
+(************
+Fixpoint lamDepth (t:Term) : nat :=
+  match t with
+    | TLambda _ body => S (lamDepth body)
+    | _ => 0
+  end.
+
+Fixpoint applyBranchToProof (n:nat) (br:Term) : Term :=
+  match n with
+    | 0 => br
+    | S m => match br with
+               | TLambda _ body => applyBranchToProof m (instantiate TProof 0 body)
+               | x => x
+             end
+  end.
+ ***********************)
+
+Fixpoint m_Proofs m : Terms :=
+  match m with
+    | 0 => tnil
+    | S n => tcons TProof (m_Proofs n)
+  end.
+Fixpoint applyBranchToProof nargs (br:Term) : Term :=
+  match nargs with
+    | 0 => br
+    | S m => mkApp br (tcons TProof (m_Proofs m))
+  end.
+
+Function L2Term_Term (t:L2Term) : Term :=
+  match t with
+    | L2.compile.TRel n => TRel n
+    | L2.compile.TSort srt => TSort srt
+    | L2.compile.TProof t => TProof
+    | L2.compile.TCast tm => TCast (L2Term_Term tm)
+    | L2.compile.TProd nm bod => TProd nm (L2Term_Term bod)
+    | L2.compile.TLambda nm bod => TLambda nm (L2Term_Term bod)
+    | L2.compile.TLetIn nm dfn bod =>
+      TLetIn nm (L2Term_Term dfn) (L2Term_Term bod)
+    | L2.compile.TApp fn arg args =>
+      TApp (L2Term_Term fn) (L2Term_Term arg) (L2Terms_Terms args)
+    | L2.compile.TConst pth => TConst pth
+    | L2.compile.TAx => TAx
+    | L2.compile.TInd ind => TInd ind
+    | L2.compile.TConstruct ind m arty => TConstruct ind m arty
+    | L2.compile.TCase ((_, _, nargs) as m) mch brs =>
+      match L2Term_Term mch, L2Terms_Terms brs, nargs with
+          | TProof, tunit Br, cons n nil => applyBranchToProof n Br
+          | Mch, Brs, _ => TCase m Mch Brs
+      end
+    | L2.compile.TFix defs m => TFix (L2Defs_Defs defs) m
+    | L2.compile.TWrong => TWrong
+  end
+with L2Terms_Terms (ts:L2Terms) : Terms :=
+       match ts with
+         | L2.compile.tnil => tnil
+         | L2.compile.tcons u us => tcons (L2Term_Term u) (L2Terms_Terms us)
+       end
+with L2Defs_Defs (ds:L2Defs) : Defs :=
+       match ds with
+         | L2.compile.dnil => dnil
+         | L2.compile.dcons nm tm m ds =>
+           dcons nm (L2Term_Term tm) m (L2Defs_Defs ds)
+       end.
+(****
+Functional Scheme L2Term_Term_ind' := Induction for L2Term_Term Sort Prop
+with L2Terms_Terms_ind' := Induction for L2Terms_Terms Sort Prop
+with L2Defs_Defs_ind' := Induction for L2Defs_Defs Sort Prop.
+Combined Scheme L2Term_TermEvalsDEvals_ind
+         from L2Term_Term_ind', L2Terms_Terms_ind', L2Defs_Defs_ind'.
+***)
+
+(** environments and programs **)
+Function L2EC_EC (ec:L2EC) : envClass Term :=
+  match ec with
+    | ecTrm t => ecTrm (L2Term_Term t)
+    | ecTyp _ n itp => ecTyp Term n itp
+  end.
+
+Definition L2Env_Env: L2Env -> environ Term :=
+  List.map (fun (nmec: string * L2EC) => (fst nmec, L2EC_EC (snd nmec))).
+
+Definition L2Pgm_Program (p:L2Pgm) : Program Term:=
+  {| env:= L2Env_Env (env p);
+     main:= L2Term_Term (main p) |}.
+
+
+(*** from L2 to L2_5 ***)
+Definition program_Program (p:program) : Program Term :=
+  L2Pgm_Program (L2.compile.program_Program p).
+
+(***
+Definition term_Term (e:AstCommon.environ L2Term) (t:term) : Term :=
+  L2Term_Term (L2.compile.term_Term e t).
+***)
